LeanAntithesis.lean
@@ -10,3 +10,4 @@ import LeanAntithesis.Logic.LinearTactic
 import LeanAntithesis.Math.Examples
 import LeanAntithesis.Math.ComplementedSet
 import LeanAntithesis.Math.Equivalence
+import LeanAntithesis.Math.Deriving
